until keyschedule

src/tls/Epochs.fst
@@ -2,6 +2,7 @@ module Epochs
 
 open FStar.Heap
 open FStar.HyperHeap
+open FStar.HyperStack
 open FStar.Seq
 open FStar.Monotonic.RRef
 open FStar.Monotonic.Seq
@@ -17,11 +18,13 @@ open StAE
 open Negotiation
 
 module HH = FStar.HyperHeap
+module HS = FStar.HyperStack
+module MR = FStar.Monotonic.RRef
 module MS = FStar.Monotonic.Seq
 module SeqP = FStar.SeqProperties
 
 // relocate?
-type fresh_subregion r0 r h0 h1 = fresh_region r h0 h1 /\ extends r r0
+type fresh_subregion r0 r h0 h1 = stronger_fresh_region r h0 h1 /\ extends r r0
 
 type epoch_region_inv (#i:id) (hs_rgn:rgn) (r:reader (peerId i)) (w:writer i) =
   disjoint hs_rgn (region w)                  /\
@@ -108,7 +111,7 @@ noeq type epochs (r:rgn) (n:TLSInfo.random) =
 	    write: epoch_ctr r es ->
 	    epochs r n
 
-let containsT (#r:rgn) (#n:TLSInfo.random) (es:epochs r n) (h:HH.t) =
+let containsT (#r:rgn) (#n:TLSInfo.random) (es:epochs r n) (h:mem) =
     MS.i_contains (MkEpochs.es es) h 
 
 val alloc_log_and_ctrs: #a:Type0 -> #p:(seq a -> Type0) -> r:HH.rid ->
@@ -118,7 +121,7 @@ val alloc_log_and_ctrs: #a:Type0 -> #p:(seq a -> Type0) -> r:HH.rid ->
      (requires (fun h -> p Seq.createEmpty))
      (ensures (fun h0 x h1 ->
        modifies_one r h0 h1
-       /\ modifies_rref r !{} h0 h1
+       /\ modifies_rref r !{} (HS.HS.h h0) (HS.HS.h h1)
        /\ (let (|is, c1, c2|) = x in
 	  i_contains is h1
 	  /\ m_contains c1 h1
@@ -137,8 +140,9 @@ val incr_epoch_ctr: #a:Type0 -> #p:(seq a -> Type0) -> #r:HH.rid -> #is:MS.i_seq
 		  -> ST unit
    (requires (fun h -> 1 + m_sel h ctr < Seq.length (i_sel h is)))
    (ensures (fun h0 _ h1 ->
+                  let ctr_as_hsref = MR.as_hsref ctr in
 		  modifies_one r h0 h1
-		  /\ modifies_rref r !{as_ref (as_rref ctr)} h0 h1
+		  /\ modifies_rref r !{as_ref ctr_as_hsref} (HS.HS.h h0) (HS.HS.h h1)
 		  /\ m_sel h1 ctr = m_sel h0 ctr + 1))
 let incr_epoch_ctr #a #p #r #is ctr =
   m_recall ctr;
@@ -149,22 +153,23 @@ let incr_epoch_ctr #a #p #r #is ctr =
        
 val epochs_init: r:rgn -> n:TLSInfo.random -> ST (epochs r n)
        (requires (fun h -> True))
-       (ensures (fun h0 x h1 -> modifies_one r h0 h1 /\ modifies_rref r !{} h0 h1))
+       (ensures (fun h0 x h1 -> modifies_one r h0 h1 /\ modifies_rref r !{} (HS.HS.h h0) (HS.HS.h h1)))
 let epochs_init (r:rgn) (n:TLSInfo.random) =
   let (| esref, c1, c2 |) = alloc_log_and_ctrs #(epoch r n) #(epochs_inv #r #n) r in
   MkEpochs esref c1 c2
 
-inline let incr_pre #r #n (es:epochs r n) (proj:(es:epochs r n -> Tot (epoch_ctr r (MkEpochs.es es)))) h : GTot Type0 =
+unfold let incr_pre #r #n (es:epochs r n) (proj:(es:epochs r n -> Tot (epoch_ctr r (MkEpochs.es es)))) h : GTot Type0 =
   let ctr = proj es in
   let cur = m_sel h ctr in
   cur + 1 < Seq.length (i_sel h (MkEpochs.es es))
 
-inline let incr_post #r #n (es:epochs r n) (proj:(es:epochs r n -> Tot (epoch_ctr r (MkEpochs.es es)))) h0 (_:unit) h1 : GTot Type0 =
+unfold let incr_post #r #n (es:epochs r n) (proj:(es:epochs r n -> Tot (epoch_ctr r (MkEpochs.es es)))) h0 (_:unit) h1 : GTot Type0 =
   let ctr = proj es in
   let oldr = m_sel h0 ctr in
   let newr = m_sel h1 ctr in
+  let ctr_as_hsref = MR.as_hsref ctr in
   modifies_one r h0 h1
-  /\ HH.modifies_rref r !{HH.as_ref (as_rref ctr)} h0 h1
+  /\ HH.modifies_rref r !{HH.as_ref (MkRef.ref ctr_as_hsref)} (HS.HS.h h0) (HS.HS.h h1)
   /\ newr = oldr + 1
 
 val add_epoch: #r:rgn -> #n:TLSInfo.random ->
@@ -173,9 +178,10 @@ val add_epoch: #r:rgn -> #n:TLSInfo.random ->
 	   let is = MkEpochs.es es in
 	   epochs_inv #r #n (SeqP.snoc (i_sel h is) e)))
        (ensures (fun h0 x h1 -> 
-		   let es = MkEpochs.es es in 
+		   let es = MkEpochs.es es in
+		   let es_as_hsref = MR.as_hsref es in
  		   modifies_one r h0 h1  
- 		   /\ modifies_rref r !{as_ref (as_rref es)} h0 h1
+ 		   /\ modifies_rref r !{as_ref es_as_hsref} (HS.HS.h h0) (HS.HS.h h1)
  		   /\ i_sel h1 es == SeqP.snoc (i_sel h0 es) e))
 let add_epoch #r #n (MkEpochs es _ _) e = 
     MS.i_write_at_end es e
@@ -196,13 +202,13 @@ let ctr (#r:_) (#n:_) (e:epochs r n) (rw:rw) = match rw with
   | Reader -> e.read
   | Writer -> e.write
 
-val readerT: #rid:rgn -> #n:TLSInfo.random -> e:epochs rid n -> HH.t -> GTot (epoch_ctr_inv rid (get_epochs e))
-let readerT #rid #n (MkEpochs es r w) (h:HH.t) = m_sel h r
+val readerT: #rid:rgn -> #n:TLSInfo.random -> e:epochs rid n -> mem -> GTot (epoch_ctr_inv rid (get_epochs e))
+let readerT #rid #n (MkEpochs es r w) (h:mem) = m_sel h r
 
-val writerT: #rid:rgn -> #n:TLSInfo.random -> e:epochs rid n -> HH.t -> GTot (epoch_ctr_inv rid (get_epochs e))
-let writerT #rid #n (MkEpochs es r w) (h:HH.t) = m_sel h w
+val writerT: #rid:rgn -> #n:TLSInfo.random -> e:epochs rid n -> mem -> GTot (epoch_ctr_inv rid (get_epochs e))
+let writerT #rid #n (MkEpochs es r w) (h:mem) = m_sel h w
 
-inline let get_ctr_post (#r:rgn) (#n:TLSInfo.random) (es:epochs r n) (rw:rw) h0 (i:int) h1 = 
+unfold let get_ctr_post (#r:rgn) (#n:TLSInfo.random) (es:epochs r n) (rw:rw) h0 (i:int) h1 = 
   let epochs = MkEpochs.es es in
   h0 == h1
   /\ i = m_sel h1 (ctr es rw)
@@ -220,7 +226,7 @@ let get_ctr (#r:rgn) (#n:TLSInfo.random) (es:epochs r n) (rw:rw)
 let get_reader (#r:rgn) (#n:TLSInfo.random) (es:epochs r n) = get_ctr es Reader
 let get_writer (#r:rgn) (#n:TLSInfo.random) (es:epochs r n) = get_ctr es Writer
 
-let epochsT #r #n (es:epochs r n) (h:HH.t) = MS.i_sel h (MkEpochs.es es)
+let epochsT #r #n (es:epochs r n) (h:mem) = MS.i_sel h (MkEpochs.es es)
   
 let get_current_epoch (#r:_) (#n:_) (e:epochs r n) (rw:rw)
   : ST (epoch r n)
